

→ Angle bet. two vectors =  $\cos^{-1} \left[ \frac{(x, y)}{\|x\|_2 \|y\|_2} \right]$

→ Properties of scaled norm:

- Should be real & non-negative
- $\|x\| = 0 \Leftrightarrow x = 0$
- $\|\alpha x\| = |\alpha| \|x\|$
- $\|x + y\| \leq \|x\| + \|y\|$

→  $|\langle x, y \rangle| \leq \|x\|_2 \|y\|_2$  (Cauchy-Schwarz inequality)

→  $\|A\|_1 = \max_{1 \leq i \leq m} (\sum_{j=1}^n |a_{ij}|)$

→  $\|A\|_\infty = \max_{1 \leq j \leq n} (\sum_{i=1}^m |a_{ij}|)$

→ If  $A = uv^T$ ,  $\|A\|_2 = \|u\|_2 \|v\|_2$  (when  $x = \frac{v}{\|v\|}$ )

→  $\|AB\|_p \leq \|A\|_p \|B\|_p$

$$\|A\|_F = \sqrt{\sum_{i=1}^m \sum_{j=1}^n |a_{ij}|^2} = \sqrt{\text{tr}(AA^T)} = \sqrt{\text{tr}(A^T A)} = \sqrt{\sum_{i=1}^m \|a_i\|_2^2}$$

$$A = U \Sigma V^T, \quad U \in \mathbb{R}^{m \times m}, \text{ orthogonal}$$

$$\Sigma \in \mathbb{R}^{m \times n}, \text{ diagonal}$$

$$V^T \in \mathbb{R}^{n \times n}, \text{ orthogonal}$$

$$\|A\|_2 = \sigma_1, \quad \|A\|_F = \sqrt{\sigma_1^2 + \dots + \sigma_n^2}$$

→ Orthogonal transformation of the feature space.

→ Consider a data matrix  $A \in \mathbb{R}^{m \times n}$  (no. of experiments, particular measurement)

- 1) Move the matrix 0-centered by subtracting the mean of the coln. from each element in the coln.
- 2) Variance of the coln. =  $\frac{E(x^2) - (E(x))^2}{m} = \frac{\|a_j\|_2^2}{m}$
- 3) Hence, total variance,  $T = \|a_1\|_2^2 + \dots + \|a_n\|_2^2$

$$= \|A\|_F^2 = \sigma_1^2 + \sigma_2^2 + \dots + \sigma_n^2$$

Biggest contributor to the variance

→ To get the direction with highest variance, we need to find a vector  $\hat{w}_1$  s.t.

$$t_1 = A \hat{w}_1, \quad \|t_1\|_2 \text{ is maximised. The solution is } \hat{w}_1 = v_1.$$

$$t_1 = A v_1 = \sum_{i=1}^n u_i \sigma_i v_i^T v_1 \quad [v_i^T v_1 = \begin{cases} 0, & i \neq 1 \\ 1, & i = 1 \end{cases}]$$

$$= u_1 \sigma_1 v_1^T v_1$$

$$= \sigma_1 u_1$$

→ Similarly,  $t_2 = \sigma_2 u_2$ , where  $t_2$  is the direction along second highest variance.

Eigen Decomposition

→  $A = X \Lambda X^{-1}$ ,  $\Lambda$  is a diagonal matrix containing eigenvalues and  $X$  is a matrix comprising of the respective eigenvectors

→ Characteristic polynomial ( $P_A$ ):  $P_A(\lambda) = \det(A - \lambda I)$

→ Eigenvectors are essentially Nullspace of  $(A - \lambda I)$ . Hence,  $(A - \lambda I)$  must be a rank-deficient (singular) matrix, with  $\det(A - \lambda I) = 0$

→ Geometric multiplicity of  $\lambda$ : No. of L.I. eigenvectors associated with an eigenvalue  $\lambda$ .

→ If  $\lambda$  corresponds to two eigenvectors  $v_1 \in V_1$ , any vector  $x = \alpha_1 v_1 + \alpha_2 v_2$  will be an eigenvector of  $A$ .

$$Ax = A(\alpha_1 v_1 + \alpha_2 v_2) = \alpha_1 A v_1 + \alpha_2 A v_2 = \alpha_1 \lambda v_1 + \alpha_2 \lambda v_2 = \lambda (\alpha_1 v_1 + \alpha_2 v_2) = \lambda x \text{ (shown)}$$

Similarity Transformation

→ If  $X \in \mathbb{R}^{m \times m}$  is non-singular,  $XAX^{-1}$  is an analogous similarity transformation of  $A$ .

→ Two matrices  $A$  &  $B$  are said to be similar if there exists a similarity transformation bet. them, i.e.  $B = XAX^{-1}$ .

→  $A$  &  $B$  will have same eigenvalues & geometric multiplicities

$$P_B(\lambda) = \det(\lambda I - XAX^{-1})$$

$$= \det(\lambda X X^{-1} I X^{-1} - X A X^{-1})$$

$$= \det(X(\lambda I - A)X^{-1})$$

$$= \det(X) \det(\lambda I - A) \det(X^{-1})$$

$$= \det(X) \det(\lambda I - A) \frac{1}{\det(X)} \text{ (shown)}$$

\* Egn. value may not be the same for  $A$  &  $B$

$$\rightarrow \text{Absolute cond. no. } \hat{\kappa} = \frac{\|Sf\|}{\|Sx\|} = \frac{\|S(x) Sx\|}{\|Sx\|} = \|S(x)\|$$

$$\rightarrow \text{Relative cond. no.} = \frac{\|Sf\|}{\|f\|} \div \frac{\|Sx\|}{\|x\|} = \frac{\|S(x)\| \|x\|}{\|f\|}$$

$$\rightarrow \kappa(A) = \frac{\sigma_1}{\sigma_m} = \sqrt{\frac{\lambda_{\max}(A^T A)}{\lambda_{\min}(A^T A)}}$$

$$\rightarrow \kappa^R(A) = \|A\| \|A^+\|, \text{ where } \|A^+\| = (A^T A)^{-1} A^T$$

→ For a backward stable algo,  $f(\hat{x}) = \tilde{f}(x)$

→ Projector matrix  $P$ , must be:

$$\rightarrow P^2 = P \text{ (idempotent)} \rightarrow P x - v \in \text{Null}(P)$$

$$\rightarrow \text{Square matrix} \rightarrow \text{Rank-deficient}$$

$$\rightarrow P x = x \quad \forall x \in \text{Range}(P) \rightarrow \text{Symmetrical}$$

→ If  $P$  is a projector, so is  $(I - P)$ . This is the complementary projector of  $P$ .

→ Let us solve  $Ax = b$  has no soln., we can solve  $Ax = Pb$  instead.  $P$  projects  $b$  onto the coln. space of  $A$ , which makes this eqn. solvable

$$\text{Hence, } P = A(A^T A)^{-1} A^T$$

→ If  $L$  is an orthogonal projector so is  $(I - P)$

$$\rightarrow \text{If } A \text{ is orthogonal, } P = A(A^T A)^{-1} A^T = AA^T$$

→ Projection & SVD: If  $A = U \Sigma V^T$ ,  $U$  forms an orthonormal basis of  $A$ . Hence, the projection matrix corresponding to  $A$ ,  $P = Q(Q^T Q)^{-1} Q^T = QQ^T$

Symmetric +ve Definite Matrices (SPD)

→ Properties

$$\rightarrow A = A^T$$

$$\rightarrow (\hat{x}, \hat{y}) = (x, y) \quad \forall x, y \in \mathbb{R}^m$$

$$\rightarrow x^T A x > 0, \quad \forall x \in \mathbb{R}^m$$

→ If  $A$  is S.P.D. &  $X \in \mathbb{R}^{m \times n}$  is full rank, then  $X^T A X$  is also S.P.D.

→ All eigenvalues are +ve for any S.P.D.

Cholansky Decomposition

$$\rightarrow \text{If } A \text{ is S.P.D., } A \text{ can be decomposed s.t. } A = R^T R$$

→  $n^3/3$  FLOPs

Linear Least Squares

→ If  $Ax = b$  is over-determined, we can solve for  $A^T A \hat{x} = A^T b$  instead. This shall minimise the residual, i.e.  $\|r\|_2$ , where  $r = Ax - b$

$$A \hat{x} = Pb \quad \text{|| get } b \text{ to coln. space of } A$$

$$\hat{x} = A(A^T A)^{-1} A^T b \Rightarrow \hat{x} = (A^T A)^{-1} A^T b$$

Soln. by Cholansky decomposition: → Soln. by QR factorisation

$$A^T A \hat{x} = A^T b$$

$$R^T R \hat{x} = A^T b$$

$$R^T w = A^T b \quad \text{|| let } w = R \hat{x}$$

$$\downarrow \text{Solve for } w$$

$$R \hat{x} = w$$

$$\downarrow \text{Solve for } \hat{x}$$

$$\hat{x}$$

Soln with SVD

$$A \hat{x} = Pb$$

$$U \Sigma V^T \hat{x} = U U^T b$$

$$\Sigma V^T \hat{x} = U^T b$$

$$\Sigma \hat{x} = U^T b \quad \text{|| let } V^T \hat{x} = \hat{x}$$

$$\downarrow \text{Solve for } \hat{x}$$

$$\hat{x}$$

Algo	Work
Cholansky	$mn^2 + n^3/3$
QR (Householder)	$2mn^2 - 2n^3/3$
SVD	$2mn^2 + 11n^3$

Backward stability:  
 $\tilde{f}(x) = f(x + \delta x)$   
 Forward stability:  
 $\|f(x) - \tilde{f}(x)\| = O(\epsilon_m)$

→  $Q$ : matrix w/ orthonormal cols. →  $R$ : UTM

→ Gram-Schmidt orthogonalisation:

$$\underline{v}_j = \underline{a}_j - (\underline{q}_1^T \underline{a}_j) \underline{q}_1 - \dots - (\underline{q}_{j-1}^T \underline{a}_j) \underline{q}_{j-1}$$

$$\underline{q}_j = \frac{\underline{v}_j}{\|\underline{v}_j\|_2}$$

Hence  $\underline{q}_n = \frac{\underline{a}_n - \sum_{i=0}^{n-1} r_{in} \underline{q}_i}{r_{nn}}$ , where  $r_{ij} = \begin{cases} \underline{v}_i^T \underline{a}_j, & i \neq j \\ \|\underline{a}_j - \sum_{i=1}^{j-1} r_{ij} \underline{q}_i\|_2, & i=j \end{cases}$

→ Modified Gram Schmidt

→ Gram Schmidt with projector:  $\underline{q}_n = \frac{P_n \underline{a}_n}{\|P_n \underline{a}_n\|}$ , where

$$P_n = I - \sum_{i=0}^{n-1} \underline{q}_i \underline{q}_i^T = I - \hat{Q}_{j-1} \hat{Q}_{j-1}^T$$

→ Modified Gram-Schmidt:

$$P_n \underline{a}_n = (I - \sum_{i=0}^{n-1} \underline{q}_i \underline{q}_i^T) \underline{a}_n = \left[ \prod_{i=0}^{n-1} (I - \underline{q}_i \underline{q}_i^T) \right] \underline{a}_n$$

for  $j=1 \rightarrow n$ :

$$\underline{v}_j^{(1)} = \underline{a}_j$$

$$\underline{v}_j^{(2)} = P_{\perp \underline{q}_1} \underline{a}_j = (I - \underline{q}_1 \underline{q}_1^T) \underline{a}_j = \underline{v}_j^{(1)} - \underline{q}_1 \underline{q}_1^T \underline{v}_j^{(1)}$$

$$\underline{v}_j^{(3)} = P_{\perp \underline{q}_2} \underline{a}_j = \underline{v}_j^{(2)} - \underline{q}_2 \underline{q}_2^T \underline{v}_j^{(2)}$$

$$\underline{v}_j^{(j)} = \underline{v}_j^{(j-1)} - \underline{q}_{j-1} \underline{q}_{j-1}^T \underline{v}_j^{(j-1)}$$

$$\underline{q}_j = \frac{\underline{v}_j^{(j)}}{\|\underline{v}_j^{(j)}\|_2}$$

→ Householder Triangularisation

→ Perform transformations to convert  $A$  to  $R$ :

$$Q_n \dots Q_1 A = R$$

$$Q_n = \begin{bmatrix} I_{(n-1) \times (n-1)} & 0 \\ 0 & \hat{F}_{(m-n+1) \times (m-n+1)} \end{bmatrix}_{m \times m}$$

memo: that prev cols. are not changed. must be an orthogonal matrix

→ Let  $\underline{\hat{x}} = \begin{bmatrix} - \\ - \\ - \\ - \end{bmatrix}$ ,  $\underline{F}$  should be s.t.  $\underline{F} \underline{x} = \begin{bmatrix} 0 \\ 0 \\ 0 \\ 0 \end{bmatrix} = \|\underline{x}\| \cdot \underline{e}_j$

Hence,  $\underline{y} = \underline{F} \underline{x} = (I - 2 \underline{u} \underline{u}^T) \underline{x}$ , where  $\underline{u} = -\frac{\underline{v}}{\|\underline{v}\|}$

where  $\underline{v} = \|\underline{x}\|_2 \underline{e}_j - \underline{x}$

Algo: for  $k=1 \rightarrow n$ :

$\underline{x} = A(x=m, k)$  // row  $k$  to column in the  $k^{\text{th}}$  col.

$\underline{v}_k = \text{sgn}(\underline{x}_k) \cdot \|\underline{x}\|_2 \underline{e}_k + \underline{x}$

$\underline{u}_k = \frac{\underline{v}_k}{\|\underline{v}_k\|}$

$A(k:m, k:n) \leftarrow 2 \underline{u}_k \underline{u}_k^T A(k:m, k:n)$

Algo	FLOPs	Stability	Error
CGS	$2mn^2$	Unstable	$O(\kappa(A)^2 \cdot \epsilon_m)$
MGS	"	Baumwilt stable	$O(\kappa(A) \cdot \epsilon_m)$
Householder	$2mn^2 - \frac{2}{3}n^3$	"	$O(\epsilon_m)$

## Linear Least Squares

Either  $m \geq n$  &  $\text{rank}(A) < n$ , or  $m < n$

$$A \underline{x} = \underline{b}$$

$$\underline{U} \underline{\Sigma} \underline{V}^T \underline{x} = \underline{b}$$

$$\underline{U}^T \underline{U} \underline{\Sigma} \underline{V}^T \underline{x} = \underline{U}^T \underline{b}$$

$$\underline{V}^T \underline{x} = \underline{\Sigma}^{-1} \underline{U}^T \underline{b}$$

Let  $\underline{x} = \underline{V}_1 \underline{y} + \underline{V}_2 \underline{z}$ , where  $\underline{V} = \begin{bmatrix} \underline{V}_1 & \underline{V}_2 \end{bmatrix}$

Hence  $\underline{y} = \underline{\Sigma}^{-1} \underline{U}^T \underline{b}$

Therefore  $\underline{x} = \underline{V}_1 \underline{\Sigma}^{-1} \underline{U}^T \underline{b} + \underline{V}_2 \underline{z}$

$\|\underline{x}\|_2 = \|\underline{V}_1 \underline{\Sigma}^{-1} \underline{U}^T \underline{b}\|_2 + \|\underline{V}_2 \underline{z}\|_2 = \|( \underline{V}_1 \underline{\Sigma}^{-1} \underline{U}^T \underline{b}, \underline{V}_2 \underline{z} )\|_2$

To minimise  $\|\underline{x}\|_2$ , we set  $\underline{z} = \underline{0}$

→ If  $\underline{b} \notin \text{Range}(A)$ , then we solve  $\underline{A} \underline{x} = \underline{P} \underline{b}$

In this case,  $\underline{x} = \underline{V}_1 \underline{\Sigma}^{-1} \underline{U}^T \underline{P} \underline{b} + \underline{V}_2 \underline{z}$

$= \underline{V}_1 \underline{\Sigma}^{-1} \underline{U}^T \underline{b} + \underline{V}_2 \underline{z}$

$\underline{P} = \underline{U} \underline{U}^T$

$\underline{U}^T \underline{U} = I$ , whereas  $\underline{U} \underline{U}^T$  will be a projector matrix

range(A)  
null(A)

inner product